Propagate changes in Content (WIP)

src/tls/Content.fst
@@ -19,16 +19,16 @@ open DataStream
 
 // this description is detailed enough to compute the size of the plaintext and ciphertext
 type fragment (i:id) =
-    | CT_Alert     : rg: frange i {fst rg >= 2} -> alertDescription -> fragment i // could insist we get exactly 2 bytes
-    | CT_Handshake : rg: frange i -> f: rbytes rg                  -> fragment i // concrete for now
-    | CT_CCS       : rg: frange i {fst rg >= 1}                    -> fragment i // one-byte; never encrypted or decrypted
-    | CT_Data      : rg: frange i -> f: DataStream.fragment i rg   -> fragment i // abstract
+  | CT_Alert    : rg:frange i {fst rg >= 2} -> alertDescription -> fragment i // could insist we get exactly 2 bytes
+  | CT_Handshake: rg:frange i -> f:rbytes rg                   -> fragment i // concrete for now
+  | CT_CCS      : rg:frange i {fst rg >= 1}                    -> fragment i // one-byte; never encrypted or decrypted
+  | CT_Data     : rg:frange i -> f: DataStream.fragment i rg   -> fragment i // abstract
 // for TLS 1.3
-//  | CT_EncryptedHandshake : rg: frange i -> f: Handshake.fragment i rg -> fragment i // abstract
-//  | CT_EarlyData : rg: frange i -> f: DataStream.fragment i rg -> fragment i // abstract
+//  | CT_EncryptedHandshake : rg:frange i -> f:Handshake.fragment i rg  -> fragment i // abstract
+//  | CT_EarlyData          : rg:frange i -> f:DataStream.fragment i rg -> fragment i // abstract
 
 // move to Seq?
-val split: #a: Type -> s:seq a {Seq.length s > 0} -> Tot(seq a * a)
+private val split: #a: Type -> s:seq a {Seq.length s > 0} -> Tot(seq a * a)
 let split #a s =
   let last = Seq.length s - 1 in
   Seq.slice s 0 last, Seq.index s last
@@ -40,74 +40,72 @@ let split #a s =
 // Ghost projection from low-level multiplexed fragments to application-level deltas
 // Some fragments won't parse; they are ignored in the projection. 
 // We may prove that they are never written on authentic streams.
-val project: i:id -> fs:seq (fragment i) -> Tot(seq (DataStream.delta i))
+val project: i:id -> fs:seq (fragment i) -> Tot (seq (DataStream.delta i))
   (decreases %[Seq.length fs]) // not-quite-stuctural termination
 #reset-options
 let rec project i fs =
   if Seq.length fs = 0 then Seq.createEmpty
   else
-      let fs, f = split #(fragment i) fs in
-      let ds = project i fs in
-      match f with
-      | CT_Data rg d -> 
-	let d : pre_fragment i = d in //A widening coercion as a proof hint, unpacking (d:fragment i (frange i)) to a pre_fragment i
-	snoc ds (DataStream.Data d)   //so that it can be repackaged as a fragment i fragment_range
-      | CT_Alert ad  -> snoc ds (DataStream.Alert ad)
-      | _            -> ds  // other fragments are internal to TLS
+    let fs, f = split #(fragment i) fs in
+    let ds = project i fs in
+    match f with
+    | CT_Data rg d ->
+      let d:pre_fragment i = d in //A widening coercion as a proof hint, unpacking (d:fragment i (frange i)) to a pre_fragment i
+      snoc ds (DataStream.Data d)   //so that it can be repackaged as a fragment i fragment_range
+    | CT_Alert rg ad -> snoc ds (DataStream.Alert ad)
+    | _ -> ds	 // other fragments are internal to TLS
 
 // try out a few lemmas
 // we may also need a projection that takes a low-level pos and yields a high-level pos
 
-val project_ignores_Handshake: i:id -> s: seq (fragment i) {Seq.length s > 0 /\ is_CT_Handshake (Seq.index s (Seq.length s - 1))} -> 
+val project_ignores_Handshake: i:id -> s:seq (fragment i) {Seq.length s > 0 /\ is_CT_Handshake (Seq.index s (Seq.length s - 1))} ->
   Lemma(project i s = project i (Seq.slice s 0 (Seq.length s - 1)))
-
 let project_ignores_Handshake i s = ()
 
 
 // --------------- parsing and formatting content types ---------------------
 
 type contentType =
-    | Change_cipher_spec
-    | Alert
-    | Handshake
-    | Application_data
+  | Change_cipher_spec
+  | Alert
+  | Handshake
+  | Application_data
 
 type contentType13 = ct: contentType { ct <> Change_cipher_spec }
 
 val ctBytes: contentType -> Tot (lbytes 1)
-let ctBytes ct =
-    match ct with
-    | Change_cipher_spec -> abyte 20z
-    | Alert              -> abyte 21z
-    | Handshake          -> abyte 22z
-    | Application_data   -> abyte 23z
+let ctBytes = function
+  | Change_cipher_spec -> abyte 20z
+  | Alert	       -> abyte 21z
+  | Handshake	       -> abyte 22z
+  | Application_data   -> abyte 23z
 
 val parseCT: pinverse_t ctBytes
 let parseCT b =
-    match cbyte b with
-    | 20z -> Correct Change_cipher_spec
-    | 21z -> Correct Alert
-    | 22z -> Correct Handshake
-    | 23z -> Correct Application_data
-    | _    -> Error(AD_decode_error, perror __SOURCE_FILE__ __LINE__ "")
+  match cbyte b with
+  | 20z -> Correct Change_cipher_spec
+  | 21z -> Correct Alert
+  | 22z -> Correct Handshake
+  | 23z -> Correct Application_data
+  | _	-> Error(AD_decode_error, perror __SOURCE_FILE__ __LINE__ "")
 
 val inverse_ct: x:_ -> Lemma
-  (requires (True)) 
+  (requires True)
   (ensures lemma_inverse_g_f ctBytes parseCT x)
   [SMTPat (parseCT (ctBytes x))]
 let inverse_ct x = ()
 
 val pinverse_ct: x:_ -> Lemma
-  (requires (True))
+  (requires True)
   (ensures (lemma_pinverse_f_g Seq.equal ctBytes parseCT x))
   [SMTPat (ctBytes (Correct._0 (parseCT x)))]
 let pinverse_ct x = ()
 
 let ctToString = function
-    | Change_cipher_spec -> "CCS"
-    | Alert              -> "Alert"
-    | Handshake          -> "Handshake"
-    | Application_data   -> "Data"
+  | Change_cipher_spec -> "CCS"
+  | Alert	       -> "Alert"
+  | Handshake	       -> "Handshake"
+  | Application_data   -> "Data"
 
 
 // --------------- conditional access to fragment representation ---------------------
@@ -115,36 +113,34 @@ let ctToString = function
 let ccsBytes = abyte 1z
 
 val ghost_repr: #i:id -> fragment i -> GTot bytes
-let ghost_repr #i f =
-  match f with
+let ghost_repr #i = function
   // FIXME: without the #i, extraction crashes
-  | CT_Data rg d      -> DataStream.ghost_repr #i d
-  | CT_Handshake rg f -> f
-  | CT_CCS            -> ccsBytes
-  | CT_Alert ad       -> Alert.alertBytes ad
+  | CT_Data _ d      -> DataStream.ghost_repr #i d
+  | CT_Handshake _ f -> f
+  | CT_CCS _         -> ccsBytes
+  | CT_Alert _ ad    -> Alert.alertBytes ad
 
-val repr: i:id{ ~(safeId i)} -> p:fragment i -> Tot (b:bytes {b = ghost_repr #i p})
-let repr i f =
-  match f with
+val repr: i:id{ ~(safeId i) } -> p:fragment i -> Tot (b:bytes {b = ghost_repr #i p})
+let repr i = function
   // FIXME: same thing
-  | CT_Data rg d      -> DataStream.repr #i rg d
-  | CT_Handshake rg f -> f
-  | CT_CCS            -> ccsBytes
-  | CT_Alert ad       -> Alert.alertBytes ad
+  | CT_Data rg d     -> DataStream.repr #i rg d
+  | CT_Handshake _ f -> f
+  | CT_CCS _         -> ccsBytes
+  | CT_Alert _ ad    -> Alert.alertBytes ad
 
-let ct (i:id) (f:fragment i): contentType =
-  match f with
-  | CT_Data rg d      -> Application_data
-  | CT_Handshake rg f -> Handshake
-  | CT_CCS            -> Change_cipher_spec
-  | CT_Alert ad       -> Alert
+val ct: i:id -> fragment i -> Tot contentType
+let ct i = function
+  | CT_Data _ _      -> Application_data
+  | CT_Handshake _ _ -> Handshake
+  | CT_CCS _         -> Change_cipher_spec
+  | CT_Alert _ _     -> Alert
 
-let rg (i:id) (f:fragment i): frange i =
-  match f with
+val rg: i:id -> fragment i -> Tot (frange i)
+let rg i = function
   | CT_Data rg _      -> rg
   | CT_Handshake rg _ -> rg
-  | CT_CCS            -> point 1 
-  | CT_Alert _        -> point 2
+  | CT_CCS rg         -> rg
+  | CT_Alert rg _     -> rg
 
 let ct_rg i f = ct i f, rg i f
 
@@ -152,25 +148,20 @@ let ct_rg i f = ct i f, rg i f
 
 let fragmentRepr (#i:id) (ct:contentType) (rg:frange i) (b:rbytes rg) = 
   match ct with 
-    | Change_cipher_spec -> b2t(op_Equality #bytes b ccsBytes)
-    | Alert              -> rg = point 2 /\ is_Correct (Alert.parse b)
-    | _                  -> True
+  | Change_cipher_spec -> 1 <= fst rg /\ b = ccsBytes
+  | Alert              -> 2 <= fst rg /\ length b = 2 /\ is_Correct (Alert.parse b)
+  | _                  -> True
 
-val mk_fragment: i:id{ ~(authId i)} -> ct:contentType -> rg:frange i -> b:rbytes rg { fragmentRepr ct rg b } ->
+val mk_fragment: i:id{ ~(authId i) } -> ct:contentType -> rg:frange i -> b:rbytes rg { fragmentRepr ct rg b } ->
   Tot (p:fragment i {b = ghost_repr p})
 let mk_fragment i ct rg b =
-    match ct with
-    | Application_data   -> CT_Data      rg (DataStream.mk_fragment #i rg b)
-    | Handshake          -> CT_Handshake rg b
-    | Change_cipher_spec -> CT_CCS 
-    | Alert              -> CT_Alert     (match Alert.parse b with | Correct ad -> ad)
+  match ct with
+  | Application_data   -> CT_Data      rg (DataStream.mk_fragment #i rg b)
+  | Handshake          -> CT_Handshake rg b
+  | Change_cipher_spec -> CT_CCS       rg
+  | Alert              -> CT_Alert     rg (match Alert.parse b with | Correct ad -> ad)
 
-(*
-val mk_ct_rg: 
-  i:id{ ~(authId i)} -> 
-  ct:contentType -> 
-  rg:frange i ->
-  b:rbytes rg { fragmentRepr ct rg b } ->
-  Lemma ((ct,rg) = ct_rg i (mk_fragment i ct rg b))
+val mk_ct_rg: i:id{ ~(authId i) } -> ct:contentType -> rg:frange i -> b:rbytes rg { fragmentRepr ct rg b } ->
+  Lemma (requires True) (ensures (ct,rg) = ct_rg i (mk_fragment i ct rg b))
+	[SMTPat (ct_rg i (mk_fragment i ct rg b))]
 let mk_ct_rg i ct rg b = ()
-*)
